src/Exp.v
@@ -1,7 +1,7 @@
-Require Import
-  Coq.Unicode.Utf8
-  Coq.Lists.List
-  Ty.
+Require Export
+  Ty
+  Lit
+  Coq.Lists.List.
 
 From Equations Require Import Equations.
 Set Equations With UIP.
@@ -19,11 +19,16 @@ Inductive Var : Env → Ty → Type :=
 Derive Signature NoConfusion for Var.
 
 Inductive Exp Γ : Ty → Type :=
+  | Constant {τ}  : Literal τ → Exp Γ τ
+  | Seq {τ τ'}    : Exp Γ τ' → Exp Γ τ → Exp Γ τ
+  | Nil {τ}       : Exp Γ (TyList τ)
+  | Cons {τ}      : Exp Γ τ → Exp Γ (TyList τ) → Exp Γ (TyList τ)
+  | Let {τ ty}    : Exp Γ ty → Exp (ty :: Γ) τ → Exp Γ τ
+
+  (* These are the terms of the base lambda calculus *)
   | VAR {τ}       : Var Γ τ → Exp Γ τ
   | LAM {dom cod} : Exp (dom :: Γ) cod → Exp Γ (dom ⟶ cod)
-  | APP {dom cod} : Exp Γ (dom ⟶ cod) → Exp Γ dom → Exp Γ cod
-
-  .
+  | APP {dom cod} : Exp Γ (dom ⟶ cod) → Exp Γ dom → Exp Γ cod.
 
 Derive Signature for Exp.
 
@@ -32,6 +37,11 @@ End Exp.
 Arguments ZV {_ _}.
 Arguments SV {_ _ _} _.
 
+Arguments Constant {Γ τ} _.
+Arguments Seq {Γ τ τ'} _ _.
+Arguments Nil {Γ τ}.
+Arguments Cons {Γ τ} _ _.
+Arguments Let {Γ τ ty} _ _.
 Arguments VAR {Γ τ} _.
 Arguments LAM {Γ dom cod} _.
 Arguments APP {Γ dom cod} _ _.
