src/Lit.v
@@ -1,0 +1,24 @@
+Require Export
+  Ty
+  Coq.Strings.String
+  Coq.ZArith.Int
+  Coq.QArith.QArith.
+
+From Equations Require Import Equations.
+Set Equations With UIP.
+
+Section Lit.
+
+Definition UTCTime : Set := nat.
+
+Inductive Literal : Ty → Set :=
+  | LString  : string → Literal (TyPrim PrimString)
+  | LInteger : Z → Literal (TyPrim PrimInteger)
+  | LDecimal : Q → Literal (TyPrim PrimDecimal)
+  | LBool    : bool → Literal (TyPrim PrimBool)
+  | LTime    : UTCTime → Literal (TyPrim PrimTime)
+  | LUnit    : Literal (TyPrim PrimUnit).
+
+Derive NoConfusion for Literal.
+
+End Lit.
