src/Sub.v
@@ -1,6 +1,4 @@
-Require Import
-  Coq.Unicode.Utf8
-  Coq.Lists.List
+Require Export
   Ty
   Exp
   Ren.
@@ -36,6 +34,12 @@ Equations STmL {Γ Γ' τ} (s : Sub Γ Γ')
 
 Fixpoint STmExp {Γ Γ' τ} (s : Sub Γ Γ') (e : Exp Γ τ) : Exp Γ' τ :=
   match e with
+  | Constant lit    => Constant lit
+  | Seq exp1 exp2   => Seq (STmExp s exp1) (STmExp s exp2)
+  | Nil             => Nil
+  | Cons x xs       => Cons (STmExp s x) (STmExp s xs)
+  | Let binder body => Let (STmExp s binder) (STmExp (STmL s) body)
+
   | VAR v     => s _ v
   | APP e1 e2 => APP (STmExp s e1) (STmExp s e2)
   | LAM e     => LAM (STmExp (STmL s) e)
