src/Ty.v
@@ -1,4 +1,4 @@
-Require Import
+Require Export
   Coq.Unicode.Utf8.
 
 From Equations Require Import Equations.
@@ -6,15 +6,33 @@ Set Equations With UIP.
 
 Section Ty.
 
-Inductive Ty : Type :=
-  | TARR : Ty → Ty → Ty
+Inductive PrimType : Type :=
+  | PrimInteger
+  | PrimDecimal
+  | PrimTime
+  | PrimBool
+  | PrimString
+  | PrimUnit.
 
-  .
+Derive NoConfusion for PrimType.
+
+(* TODO:
+ - Row-types
+ - Modules
+ - Schemas
+ - Tables
+ - Guards
+ - Capabilities *)
+
+Inductive Ty : Type :=
+  | TyPrim : PrimType → Ty
+  | TyList : Ty → Ty
+
+  (* The arrow type is the only type in the base lambda calculus *)
+  | TyArrow : Ty → Ty → Ty.
 
 Derive NoConfusion for Ty.
 
 End Ty.
 
-Arguments TARR _ _.
-
-Infix "⟶" := TARR (at level 30, right associativity).
+Infix "⟶" := TyArrow (at level 30, right associativity).
